Update Submission.thy

homework/13/Submission.thy
@@ -2,15 +2,64 @@ theory Submission
   imports Defs
 begin
 
+fun inv_plus'_filter :: "bound \<Rightarrow> bound \<Rightarrow> bound \<Rightarrow> bool"  where
+  "inv_plus'_filter NegInf NegInf NegInf = True" |
+  "inv_plus'_filter NegInf NegInf Real = True" |
+  "inv_plus'_filter NegInf Real NegInf = True" |
+  "inv_plus'_filter PosInf PosInf PosInf = True" |
+  "inv_plus'_filter PosInf PosInf Real = True" |
+  "inv_plus'_filter PosInf Real PosInf = True" |
+  "inv_plus'_filter NaN NegInf PosInf = True" |
+  "inv_plus'_filter NaN PosInf NegInf = True" |
+  "inv_plus'_filter NaN NaN _ = True" |
+  "inv_plus'_filter NaN _ NaN = True" |
+  "inv_plus'_filter Real Real Real = True" |
+  "inv_plus'_filter _ _ _ = False"
+
 fun inv_plus' :: "bounds \<Rightarrow> bounds \<Rightarrow> bounds \<Rightarrow> (bounds * bounds)"  where
-  "inv_plus' _ = undefined"
+  "inv_plus' (B b) (B b1) (B b2) = 
+  (B {bb1 \<in> b1. \<exists>bb \<in> b. \<exists>bb2 \<in> b2. inv_plus'_filter bb bb1 bb2},
+  B {bb2 \<in> b2. \<exists>bb \<in> b. \<exists>bb1 \<in> b1. inv_plus'_filter bb bb1 bb2})"
+
+fun inv_less'_helper :: "bool \<Rightarrow> bound \<Rightarrow> bound \<Rightarrow> (bound * bound) option" where
+  "inv_less'_helper _ NaN _ = None" |
+  "inv_less'_helper _ _ NaN = None" |
+  "inv_less'_helper _ Real Real = Some (Real, Real)" |
+  "inv_less'_helper True PosInf _ = None" |
+  "inv_less'_helper True x PosInf = Some (x, PosInf)" |
+  "inv_less'_helper True _ NegInf = None" |
+  "inv_less'_helper True NegInf x = Some (NegInf, x)" |
+  "inv_less'_helper False PosInf x = Some (PosInf, x)" |
+  "inv_less'_helper False _ PosInf = None" |
+  "inv_less'_helper False x NegInf = Some (x, NegInf)" |
+  "inv_less'_helper False NegInf _ = None"
+
+fun inv_less'_filter :: "bool option \<Rightarrow> bound \<Rightarrow> bound \<Rightarrow> bool" where
+  "inv_less'_filter None NaN _ = True" |
+  "inv_less'_filter None _ NaN = True" |
+  "inv_less'_filter (Some _) NaN _ = False" |
+  "inv_less'_filter (Some _) _ NaN = False" |
+  "inv_less'_filter (Some _) Real Real = True" |
+  "inv_less'_filter (Some True) PosInf _ = False" |
+  "inv_less'_filter (Some True) _ PosInf = True" |
+  "inv_less'_filter (Some True) _ NegInf = False" |
+  "inv_less'_filter (Some True) NegInf _ = True" |
+  "inv_less'_filter (Some False) PosInf _ = True" |
+  "inv_less'_filter (Some False) _ NegInf = True" |
+  "inv_less'_filter _ _ _ = False"
 
 fun inv_less' :: "bool option \<Rightarrow> bounds \<Rightarrow> bounds \<Rightarrow> (bounds * bounds)"  where
-  "inv_less' _ = undefined"
+  "inv_less' b (B b1) (B b2) = 
+  (B {bb1 \<in> b1. \<exists>bb2 \<in> b2. inv_less'_filter b bb1 bb2},
+  B {bb2 \<in> b2. \<exists>bb1 \<in> b1. inv_less'_filter b bb1 bb2})"
 
 value "inv_plus' (B {NaN}) (B {\<infinity>\<^sup>+}) (B {\<infinity>\<^sup>-, Real}) = (B {\<infinity>\<^sup>+}, B {\<infinity>\<^sup>-})"
 value "inv_plus' (B {\<infinity>\<^sup>+,\<infinity>\<^sup>-}) (B {\<infinity>\<^sup>+, NaN}) (B {\<infinity>\<^sup>-, Real, \<infinity>\<^sup>+}) = (B {\<infinity>\<^sup>+}, B {\<infinity>\<^sup>+, Real})"
 value "inv_less' (Some True) (B {\<infinity>\<^sup>+, \<infinity>\<^sup>-}) (B {\<infinity>\<^sup>+}) = (B {\<infinity>\<^sup>-}, B {\<infinity>\<^sup>+})"
+
+lemma inv_plus'_sub:
+  assumes "inv_plus' (B A) (B A1) (B A2) = (B A1', B A2')"
+  shows "A1' \<subseteq> A1" "A2' \<subseteq> A2" using assms by auto
 
 lemma inv_plus'_sound:
     assumes "inv_plus' (B A) (B A1) (B A2) = (B A1', B A2')"
@@ -22,8 +71,43 @@ lemma inv_plus'_sound:
            | (Some PInfty, Some MInfty) \<Rightarrow> None \<in> \<gamma>_bounds (B A)
            | (Some MInfty, Some PInfty) \<Rightarrow> None \<in> \<gamma>_bounds (B A)
            | (Some i1, Some i2) \<Rightarrow> Some (i1+i2) \<in> \<gamma>_bounds (B A))"
-  shows "i1 \<in> \<gamma>_bounds (B A1') \<and> i2 \<in> \<gamma>_bounds (B A2')"
-  sorry
+    shows "i1 \<in> \<gamma>_bounds (B A1') \<and> i2 \<in> \<gamma>_bounds (B A2')"
+  apply(cases i1; cases i2)
+proof(goal_cases)
+  case 1
+  with assms show ?case by fastforce
+next
+  case (2 a)
+  with assms show ?case by fastforce
+next
+  case (3 a)
+  with assms(4) have "None \<in> \<gamma>_bounds (B A)" by(cases a, auto)
+  then have "NaN \<in> A" by auto
+  with assms have "NaN \<in> A2'"
+    apply (auto simp: 3(2))
+    using \<gamma>_bound.cases inv_plus'_filter.simps by metis
+  with 3(2) have "i2 \<in> \<gamma>_bounds (B A2')" by auto
+  moreover
+  have "\<forall>x. inv_plus'_filter NaN x NaN"
+    using inv_plus'_filter.elims(3) by blast
+  then have "\<forall>x. \<exists>bb \<in> A. \<exists>bb2 \<in> A2. inv_plus'_filter bb x bb2"
+    using \<open>NaN \<in> A\<close> \<open>NaN \<in> A2'\<close>  inv_plus'_sub assms(1) by blast
+  then obtain v where v_def: 
+    "v = (case a of ereal r \<Rightarrow> Real | PInfty \<Rightarrow> PosInf | MInfty \<Rightarrow> NegInf)" by blast
+  with assms 3 have "v \<in> A1" by(cases a, auto)
+  then have "v \<in> A1'"
+    using assms(1) \<open>\<forall>x. \<exists>bb \<in> A. \<exists>bb2 \<in> A2. inv_plus'_filter bb x bb2\<close> by auto
+  then have "i1 \<in> \<gamma>_bounds (B A1')" by(cases a, auto simp: v_def 3(1))
+  ultimately show ?case by simp
+next
+  case (4 a aa)
+  with assms show ?case apply(cases a; cases aa, auto)
+    using inv_plus'_filter.simps by blast+
+qed
+
+lemma inv_less'_sub:
+  assumes "inv_less' bv (B A1) (B A2) = (B A1', B A2')"
+  shows "A1' \<subseteq> A1" "A2' \<subseteq> A2" using assms by auto
 
 lemma inv_less'_sound:
     assumes "inv_less' bv (B A1) (B A2) = (B A1',B A2')"
@@ -33,7 +117,37 @@ lemma inv_less'_sound:
              (None, _) \<Rightarrow> None = bv
            | (_, None) \<Rightarrow> None = bv
            | (Some i1, Some i2) \<Rightarrow> Some (i1<i2) = bv)"
-  shows "i1 \<in> \<gamma>_bounds (B A1') \<and> i2 \<in> \<gamma>_bounds (B A2')"
-  sorry
+  shows "i1 \<in> \<gamma>_bounds (B A1') \<and> i2 \<in> \<gamma>_bounds (B A2')" using assms
+ apply(cases i1; cases i2)
+proof(goal_cases)
+  case 1
+  with assms show ?case by fastforce
+next
+  case (2 a)
+  with assms show ?case by fastforce
+next
+  case (3 a)
+  with assms(4) have "None = bv" by(cases a, auto)
+  with assms have "NaN \<in> A2'"
+    apply (auto simp: 3(10))
+    using \<gamma>_bound.cases inv_less'_filter.simps by metis
+  with 3(10) have "i2 \<in> \<gamma>_bounds (B A2')" by auto
+  moreover
+  have "\<forall>x. inv_less'_filter None x NaN"
+    using inv_less'_filter.elims(3) by blast
+  then have "\<forall>x. \<exists>bb2 \<in> A2. inv_less'_filter bv x bb2"
+    using \<open>None = bv\<close> \<open>NaN \<in> A2'\<close>  inv_less'_sub assms(1) by blast
+  then obtain v where v_def: 
+    "v = (case a of ereal r \<Rightarrow> Real | PInfty \<Rightarrow> PosInf | MInfty \<Rightarrow> NegInf)" by blast
+  with assms 3 have "v \<in> A1" by(cases a, auto)
+  then have "v \<in> A1'"
+    using assms(1) \<open>\<forall>x. \<exists>bb2 \<in> A2. inv_less'_filter bv x bb2\<close> by auto
+  then have "i1 \<in> \<gamma>_bounds (B A1')" by(cases a, auto simp: v_def 3(5))
+  ultimately show ?case by simp
+next
+  case (4 a aa)
+  with assms show ?case apply(cases a; cases aa, auto)
+    using inv_less'_filter.simps by blast+
+qed
 
 end
